more functor experiments

theories/Prelude.v
@@ -102,34 +102,32 @@ Proof. intros H. simp up_ren. apply congr_rcons. now apply congr_rcomp. Qed.
 (** *** Normal functors. *)
 (*********************************************************************************)
 
-(*Record encoding (Shape : Type) (size : Shape -> nat) (A : Type) : Type :=
-  { shape : Shape 
-  ; elems : vec A (size shape) 
-  }.
-Arguments shape {Shape} {size} {A} e.
-Arguments elems {Shape} {size} {A} e.*)
-
 Class NormalFunctor (F : Type -> Type) :=
   (** Usual functor stuff. *)
   { map {A B} : (A -> B) -> F A -> F B
-  ; map_id A (x : F A) : 
-      map (fun a => a) x = x
-  ; map_comp A B C (g : B -> C) (f : A -> B) (x : F A) :
-      map g (map f x) = map (fun a => g (f a)) x
+  ; map_id A (f : A -> A) (x : F A) : 
+      f =₁ id -> 
+      map f x = x
+  ; map_comp A B C (f : A -> C) (f1 : A -> B) (f2 : B -> C) (x : F A) :
+      (fun a => f2 (f1 a)) =₁ f -> 
+      map f2 (map f1 x) = map f x
   (** Encoding as a vector. *)
   ; shape : Type
   ; size : shape -> nat
   ; encode_shape {A} : F A -> shape
-  ; encode_elems {A B} : forall (f : A -> B) (x : F A), vec B (size (encode_shape x))
+  ; encode_elems {A} : forall (x : F A), vec A (size (encode_shape x))
   ; decode {A} : forall sh, vec A (size sh) -> F A
-  ; encode_decode {A B} (f : A -> B) (x : F A) : 
-      decode (encode_shape x) (encode_elems f x) = map f x
+  ; encode_decode_map {A B} (f : A -> B) (x0 : F A) : 
+      let x1 := encode_elems x0 in 
+      let x2 := vec_map f x1 in 
+      let x3 := decode (encode_shape x0) x2 in 
+      x3 = map f x0
   }.
 Arguments map F {NormalFunctor} {A} {B}.
 Arguments shape F {NormalFunctor}.
 Arguments size F {NormalFunctor} {s}.
 Arguments encode_shape F {NormalFunctor} {A}.
-Arguments encode_elems F {NormalFunctor} {A} {B}.
+Arguments encode_elems F {NormalFunctor} {A}.
 Arguments decode F {NormalFunctor} {A}.
 
 Module OptionNF.
@@ -140,9 +138,9 @@ Module OptionNF.
   encode_shape (Some _) := true ;
   encode_shape None := false.
 
-  Equations encode_elems {A B} (f : A -> B) (x : option A) : vec B (size (encode_shape x)) :=
-  encode_elems f (Some a) := [ f a ] ;
-  encode_elems f None := [].
+  Equations encode_elems {A} (x : option A) : vec A (size (encode_shape x)) :=
+  encode_elems (Some a) := [ a ] ;
+  encode_elems None := [].
     
   Equations decode {A} (sh : shape) (x : vec A (size sh)) : option A :=
   decode true  [ a ] := Some a ;
@@ -154,8 +152,8 @@ Instance option_normal_functor : NormalFunctor option :=
   Build_NormalFunctor option option_map _ _ OptionNF.shape OptionNF.size 
     (@OptionNF.encode_shape) (@OptionNF.encode_elems) (@OptionNF.decode) _.
 Proof.
-- intros A [a|] ; cbn ; reflexivity.
-- intros A B C g f [a|] ; cbn ; reflexivity.
+- intros A f [a|] H ; cbn ; rewrite ?H ; reflexivity.
+- intros A B C f f1 f2 [a|] H ; cbn ; rewrite ?H ; reflexivity.
 - intros A B f [a|] ; cbn ; reflexivity.
 Defined. 
 
@@ -166,10 +164,10 @@ Module ListNF.
   Definition encode_shape {A} (xs : list A) : shape :=
     List.length xs.
 
-  Fixpoint encode_elems {A B} (f : A -> B) (xs : list A) : vec B (size (encode_shape xs)) :=
+  Fixpoint encode_elems {A} (xs : list A) : vec A (size (encode_shape xs)) :=
     match xs with 
     | [] => vnil
-    | x :: xs => vcons (f x) (encode_elems f xs)
+    | x :: xs => vcons x (encode_elems xs)
     end. 
     
   Definition decode {A} (sh : shape) (elems : vec A (size sh)) : list A :=
@@ -181,8 +179,8 @@ Instance list_normal_functor : NormalFunctor list :=
   Build_NormalFunctor list List.map _ _ ListNF.shape ListNF.size 
     (@ListNF.encode_shape) (@ListNF.encode_elems) (@ListNF.decode) _.
 Proof.
-- intros A x. now rewrite List.map_id.
-- intros A B C g f x. now rewrite List.map_map.
+- intros A f x H. induction x ; cbn ; [reflexivity | now rewrite H, IHx].
+- intros A B C f f1 f2 x H. induction x ; cbn ; [reflexivity | now rewrite H, IHx].
 - intros A B f x. induction x ; cbn ; [reflexivity | now f_equal].
 Defined.
 
